équations d'élimination de term_altrect

theories/quotlambda_new.v
@@ -1,9 +1,10 @@
-From mathcomp.ssreflect 
-Require Import ssreflect ssrfun ssrbool ssrnat eqtype seq.
-From mathcomp.discrete Require Import tuple choice bigop fintype finfun finset generic_quotient.
-From mathcomp.fingroup Require Import perm fingroup.
+Require Import ssreflect ssrfun ssrbool ssrnat eqtype choice seq.
+Require Import bigop fintype finfun finset generic_quotient perm.
+Require Import tuple.
+Require Import fingroup.
 Require Import finmap.
 Require Import finsfun.
+Require Import Program.
 Set Implicit Arguments.
 Unset Strict Implicit.
 Unset Printing Implicit Defensive.
@@ -11,36 +12,9 @@ Unset Printing Implicit Defensive.
 Delimit Scope finperm_scope with fperm.
 Local Open Scope finperm_scope.
 Local Open Scope fset.
+Local Open Scope quotient_scope.
 
 Definition atom := nat.
-
-Section fsubset_automation.
-  Import Key.Exports.
-  
-  Context {A : keyType}.
-
-  (** Typeclass to find a proof that [R \fsubset S] given [R] and [S]. *)
-  Class is_fsubset (R : {fset A}) (S : {fset A}) :=
-    fsubset_prf : R \fsubset S.
-
-  Global Instance id_subset S : is_fsubset S S :=
-    { fsubset_prf := fsubsetAA S }.
-  
-  Global Instance left_union_subset S T U (Hl : is_fsubset S T) : is_fsubset S (T :|: U).
-  Proof. 
-      by apply/(fsubset_trans Hl)/fsubsetUl.
-  Qed.
-  
-  Global Instance right_union_subset S T U (Hl : is_fsubset S U) : is_fsubset S (T :|: U).
-  Proof. 
-      by apply/(fsubset_trans Hl)/fsubsetUr.
-  Qed.
-  
-  (** Could be extended for more complex reasoning, probably specialized to atoms and supports *)
-End fsubset_automation.
-
-Hint Mode is_fsubset + + + : typeclass_instances. 
-(* Enforce strictly structural proof search, no looping possible *)
 
 Section FinPermDef.
 
@@ -382,6 +356,14 @@ Lemma tfinpermNone a a' b :
   (b != a) && (b != a') -> (tfinperm a a') b = b.
 Proof. by case: tfinpermP => //; move ->; rewrite eqxx //= andbF. Qed.
 
+Lemma tfinpermC a b : tfinperm a b = tfinperm b a.
+Proof.
+apply/eq_finPermP => z; case: tfinpermP;
+  do ?by move ->; rewrite ?tfinpermL ?tfinpermR.
+by move => zNab; rewrite tfinpermNone // andbC.
+Qed.
+
+
 Lemma tfinsfun_id a :
   tfinsfun a a = 1.
 Proof.
@@ -389,6 +371,18 @@ apply/finsfunP => b; rewrite finsfun1.
 by case: tfinpermP; symmetry.
 Qed.
 
+Lemma tfinperm_idempotent a b :
+  (tfinperm a b) * (tfinperm a b) = 1.
+Proof.
+apply/eq_finPermP => c.
+rewrite finsfunM finsfun1 /=.
+case: tfinpermP; case: tfinpermP;
+  do ?(by move ->).  
+  - by move /andP => [/eqP ? /eqP ?]. 
+  - by move /andP => [/eqP ? /eqP ?].
+  - by rewrite eqxx => _ /andP [? ?]. 
+  - by rewrite eqxx => _ /andP [? ?]. 
+Qed.
 
 Lemma tfinperm_conj a a' (π : finPerm) :
   π * (tfinperm a a') = tfinperm (π a) (π a') * π.
@@ -399,6 +393,23 @@ rewrite ?tfinpermL ?tfinpermR ?tfinsfun_id ?finsfun1 //.
 move/andP => [ab a'b]. have [πb_out] : (π b != π a) && (π b != π a').
   by rewrite !inj_eq; do ?apply finperm_inj; apply/andP.
 by rewrite tfinpermNone.
+Qed.
+
+Lemma tfinperm_supp x y : finsupp (tfinperm x y) \fsubset [fset x;y].
+Proof.
+apply/fsubsetP => z. rewrite mem_finsupp in_fset2.
+apply contraR => /norP /andP ?. 
+by apply/eqP/tfinpermNone.
+Qed.
+
+Lemma tfinperm_disj x y S : 
+  x \notin S -> y \notin S -> [disjoint S & (finsupp (tfinperm x y))].
+Proof.
+move => xNS yNS.
+rewrite fdisjoint_sym. apply (@fdisjoint_trans _ _ [fset x;y]);
+  first exact: tfinperm_supp.                       
+apply/fdisjointP => z. rewrite in_fset2 => /orP.
+by case => /eqP ->.
 Qed.
 
 End Transpositions.
@@ -437,7 +448,7 @@ Notation swap := tfinperm.
 
 Section BasicNominalTheory.
 
-Variables (X Y : nominalType).
+Variables (W X Y Z : nominalType).
 Implicit Types (π : finPerm) (x : X).
 
 Local Notation act π := (@actN X π).
@@ -462,26 +473,60 @@ Proof. by move => x; rewrite -actM (finperm_invVP π) act1. Qed.
 Lemma act_inj π : injective (act π).
 Proof. by move => x y /(congr1 (act π^-1)); rewrite !actK. Qed.
 
-Definition equivariant1 (f : X -> Y) := forall π x, f (π \dot x)= π \dot (f x). 
-
-Definition equivariant2 (f : X -> X -> Y) := 
-  forall π x x',  f (π \dot x) (π \dot x') = π \dot (f x x').
-
 End BasicNominalTheory.
 
 Definition support (nt : nominalType) x := supp (nominal_mix nt) x.
+
+Section NominalProd.
+
+Variables (X Y : nominalType).
+Implicit Type (x : X * Y).
+
+Definition prodact π x := (π \dot x.1, π \dot x.2).
+
+Lemma prodact1 : forall x, prodact 1 x = x.
+Proof. by case => x y; rewrite /prodact !act1. Qed.
+
+Lemma prodactM π π' : forall x, prodact (π * π') x = prodact π (prodact π' x).
+Proof. by case => x y /=; rewrite /prodact !actM. Qed.
+
+Lemma prodactproper : forall x y π, x = y -> (prodact π x) = (prodact π y).
+Proof. by move => x y π ->. Qed.
+
+Definition prod_nominal_setoid_mixin := 
+  @PermSetoidMixin (X * Y) (@eq (X * Y)) prodact prodact1 prodactM prodactproper.   
+
+Lemma prodact_id (π : finPerm) x :
+     (forall a, a \in (support x.1 :|: support x.2) -> π a = a) -> prodact π x = x.
+Proof. 
+case: x => x y Hsupp. rewrite /prodact !act_id //= => a asupp; apply Hsupp;
+rewrite in_fsetU asupp ?orbT //.
+Qed.
+
+Canonical prod_nominal_mixin :=
+  @NominalMixin _ prod_nominal_setoid_mixin _ prodact_id.
+
+Canonical prod_nominal_type :=
+  NominalType prod_nominal_mixin.
+
+End NominalProd.
+
+(* Lemma strong_prodctsupport π a : *)
+(*   atomact π a = a -> (forall b, b \in fset1 a -> atomact π b = b). *)
+(* Proof. move => /= πa_eq_a b. by rewrite in_fset1 => /eqP ->. Qed. *)
+
 
 Section NominalAtoms.
 
 Implicit Types (π : finPerm) (a : atom).
 
-Local Notation atomact := (fun (π : finPerm) (a : atom) => π a).
+Definition atomact π a := π a.
 
 Lemma atomact1 : forall (a : atom), atomact 1 a = a.
-Proof. by move => a /=; rewrite finsfun1. Qed.
+Proof. by move => a /=; rewrite /atomact finsfun1. Qed.
 
 Lemma atomactM : forall π π' a, atomact (π * π') a = atomact π (atomact π' a).
-Proof. by move => π π' a /=; rewrite finsfunM. Qed.
+Proof. by move => π π' a /=; rewrite /atomact finsfunM. Qed.
 
 Lemma atomactproper : forall x y π, x = y -> (atomact π x) = (atomact π y).
 Proof. by move => x y π ->. Qed.
@@ -497,13 +542,21 @@ Lemma strong_atomactsupport π a :
   atomact π a = a -> (forall b, b \in fset1 a -> atomact π b = b).
 Proof. move => /= πa_eq_a b. by rewrite in_fset1 => /eqP ->. Qed.
 
-End NominalAtoms.
-
 Canonical atom_nominal_mixin :=
   @NominalMixin nat_choiceType atom_nominal_setoid_mixin _ atomact_id.
 
 Canonical atom_nominal_type :=
   @NominalType nat_choiceType atom_nominal_mixin.
+
+Lemma swapL a b : (swap a b) \dot a = b. 
+Proof. by rewrite /actN /= /atomact tfinpermL. Qed.
+
+Lemma swapR a b : (swap a b) \dot b = a.
+Proof. by rewrite /actN /= /atomact tfinpermR. Qed.
+
+End NominalAtoms.
+
+
 
 Section NominalAtomSubsets.
 
@@ -560,18 +613,69 @@ Proof. by apply/mem_im/finperm_inj. Qed.
 
 End NominalAtomSubsets. 
 
+Section NominalBool.
+
+Implicit Types (π : finPerm) (b : bool).
+
+Definition boolact π b := b.
+
+Lemma boolact1 : forall b, boolact 1 b = b.
+Proof. by []. Qed.
+
+Lemma boolactM : forall π π' b, boolact (π * π') b = boolact π (boolact π' b).
+Proof. by []. Qed.
+
+Lemma boolactproper : forall b b' π, b = b' -> (boolact π b) = (boolact π b').
+Proof. by move => b b' π ->. Qed. 
+
+Lemma boolact_id π b :
+  (forall a, a \in fset0 -> π a = a) -> boolact π b = b.
+Proof. by []. Qed.
+
+Definition bool_nominal_setoid_mixin := 
+  @PermSetoidMixin bool (@eq bool) boolact boolact1 boolactM boolactproper. 
+
+Canonical bool_nominal_mixin :=
+  @NominalMixin bool_choiceType bool_nominal_setoid_mixin _ boolact_id.
+
+Canonical bool_nominal_type :=
+  @NominalType bool_choiceType bool_nominal_mixin. 
+
+Lemma boolactE π b : π \dot b = b.
+Proof. by []. Qed.
+
+End NominalBool.
 
 
 Section Freshness.
 
 Variable (X : nominalType).
 
-Definition max (A : {fset atom}) := \max_(a : A) val a. 
+(* Definition max (A : {fset atom}) := \max_(a : A) val a.  *)
 
-Definition fresh (A : {fset atom}) := (max A).+1.
+Fixpoint max_list l := match l with
+                             |[::] => 0
+                             |a::q => maxn (max_list q) a
+                                           end.
+
+Definition fresh_list (l : seq atom) := (max_list l).+1.
+Definition fresh (A : {fset atom}) := fresh_list (fset_keys A). 
+(* casse l'interface, mais comment faire autrement ? *)
+
+(* Lemma fresh_notin A : fresh A \notin A. *)
+(* Proof. *)
+(* rewrite/fresh. *)
+(* suff : (forall x, x \in A -> x <= max A). *)
+(*   move => H. apply contraT. rewrite negbK => /H. by rewrite ltnn. *)
+(* move => x xA.  *)
+(* have : x = val (SeqSub xA) by []; move ->. *)
+(*   apply (@leq_bigmax A val (SeqSub xA)). *)
+(* Qed. *)
+
+Lemma freshlist_notin (s : seq atom) : (fresh_list s).+1 \notin s.
+Admitted.
 
 Lemma fresh_notin A : fresh A \notin A.
-Proof.
 Admitted.
 
 Lemma fresh_subsetnotin (A B: {fset atom}) : A \fsubset B -> fresh B \notin A. 
@@ -602,6 +706,73 @@ Qed.
 
 End Freshness.
 
+Section EquivariantFunctions.
+
+Implicit Types (W X Y Z: nominalType) (π : finPerm).
+
+Definition equivariant1 X Y (f : X -> Y) := forall π x, f (π \dot x) = π \dot (f x). 
+
+Definition equivariant2 X Y Z (f : X -> Y -> Z) := 
+  forall π x y,  f (π \dot x) (π \dot y) = π \dot (f x y).
+
+Definition equivariant3 X Y Z W (f :  X -> Y -> Z -> W) :=
+  forall π x y z, f (π \dot x) (π \dot y) (π \dot z) = π \dot (f x y z).
+
+Definition equivariant_prop X Y (R : X -> Y -> Prop) :=
+  forall π x y, R (π \dot x) (π \dot y) <-> R x y.
+
+Lemma equi_funprop X Y Z (f : X -> Y -> Z) (R : Z -> Z -> Prop) :
+  equivariant2 f -> equivariant_prop R -> 
+  equivariant_prop (fun (x : X) (y : Y * Y) => R (f x y.1) (f x y.2)). 
+Proof.
+move => equi_f equi_R π x; case => y y' /=.
+by rewrite !equi_f equi_R. 
+Qed.
+
+Lemma swap_equiv X : 
+  equivariant2 (fun (a : atom) (z : atom * X) => swap z.1 a \dot z.2).
+Proof.
+move => π a; case => b x /=. by rewrite -!actM tfinperm_conj.
+Qed.
+
+End EquivariantFunctions.
+
+Section FinitelySupportedFunctions.
+
+Implicit Types (V W X Y Z : nominalType) (π : finPerm) (S : {fset atom}).
+
+Definition function_support1 X Y (f : X -> Y) S :=
+  forall π, [disjoint S & (finsupp π)] -> forall x, π \dot (f x) = f (π \dot x).
+
+Definition finitely_supported1 X Y (f : X -> Y) := 
+  exists S, function_support1 f S.
+
+Definition function_support2 X Y Z (f : X -> Y -> Z) S :=
+  forall π, [disjoint S & (finsupp π)] -> 
+            forall x y, π \dot (f x y) = f (π \dot x) (π \dot y).
+
+Definition finitely_supported2 X Y Z (f : X -> Y -> Z) := 
+  exists S, function_support2 f S.
+
+
+Definition function_support3 X Y Z W (f : X -> Y -> Z -> W) S :=
+  forall π, [disjoint S & (finsupp π)] -> 
+            forall x y z,  π \dot (f x y z) = f (π \dot x) (π \dot y) (π \dot z).
+
+Definition finitely_supported3 X Y Z W (f : X -> Y -> Z -> W ) := 
+  exists S, function_support3 f S.
+
+Definition function_support4 X Y Z W V (f : X -> Y -> Z -> W -> V) S :=
+  forall π, [disjoint S & (finsupp π)] -> 
+            forall x y z w, 
+              π \dot (f x y z w) =
+              f (π \dot x) (π \dot y) (π \dot z) (π \dot w).
+
+Definition finitely_supported4 X Y Z W V (f : X -> Y -> Z -> W -> V) := 
+  exists S, function_support4 f S.
+
+End FinitelySupportedFunctions.
+
 Section StrongSupport.
 
 Variables (X : nominalType).
@@ -609,7 +780,7 @@ Implicit Types (x : X).
 
 (* hypothèse équivalente à : "support x" est le plus petit support de x *)
 Hypothesis strong_support : 
-  forall π x, π \dot x = x -> (forall a : atom, a \in support x -> π a = a).
+  forall x π, π \dot x = x -> (forall a : atom, a \in support x -> π a == a).
 
 Lemma equi_support : equivariant1 (@support X).
 Proof.
@@ -627,7 +798,7 @@ have : swap (val b) c \dot x = x.
   by apply fresh_subsetnotin; rewrite fsubsetU1.
 have {bx} bx : val b \in support x. by apply valP.
 move/strong_support => H. move: (H (val b) bx).
-rewrite tfinpermL => cvalb. move: (fresh1U  (im π^-1 (support (π \dot x))) (val b)).
+rewrite tfinpermL => /eqP cvalb. move: (fresh1U  (im π^-1 (support (π \dot x))) (val b)).
 by rewrite-/c -cvalb eqxx. 
 Qed.
 
@@ -637,16 +808,22 @@ Proof.
 by rewrite -[a \in _](mem_imperm π) equi_support -actM finperm_invVP act1. 
 Qed.
 
+Lemma supp_fx (Y : nominalType) (f : X -> Y) (S : {fset atom})  (fs_f : function_support1 f S) : forall (x : X), support (f x) \fsubset (S :|: support x).
+Proof.
+move => x.
+apply/fsubsetP => a. apply contraLR => aNS.
+have test : (swap a (fresh (a |: support x))) \dot x = x.
+  admit.
+
+Abort All.
+
+
 End StrongSupport.
 
 
 Section SomeAny.
 
-Variable (X : nominalType).
-
-Lemma neq_fresh (a a' : atom) :
-  (a \notin support a') = (a != a').
-Proof. by rewrite in_fset1. Qed.
+Variable (X Y : nominalType).
 
 Definition new (P : atom -> Prop) :=
   exists A : {fset atom}, forall a, a \notin A -> P a.
@@ -656,31 +833,31 @@ Notation "\new a , P" := (new (fun a:atom => P))
 Notation "a # x" := (a \notin support x)
                       (at level 0).
 
-Definition equivariant_set (R : atom -> X -> Prop) :=
-  forall (π : finPerm) a x, R (π \dot a) (π \dot x) <-> R a x. 
-
 Theorem some_any (R : atom -> X -> Prop) :
-  equivariant_set R ->
+  equivariant_prop R ->
   forall x : X, [/\
       (forall a : atom , a # x -> R a x) -> (\new a, R a x),
-      (\new a, R a x) ->  (exists2 a, a # x & R a x) &
+      (\new a, R a x) ->  R (fresh (support x)) x,
+      R (fresh (support x)) x -> (exists2 a, a # x & R a x) &
       (exists2 a, a # x & R a x)
       -> (forall a, a # x -> R a x)
     ].
 Proof.
 move => Requi; split; first by exists (support x).
-  move => [S aNSR]. exists (fresh (support x :|: S)).
-    by apply/fresh_subsetnotin/fsubsetUl.
-  apply/aNSR/fresh_subsetnotin/fsubsetUr.
-move => [a a_fresh_x rax] a' a'_fresh_x.
-case: (eqVneq a a'); first by move <-.
-move => aa'. 
-rewrite -[a'](tfinpermL a a') -[x](fresh_transp a_fresh_x a'_fresh_x) //. 
-by apply Requi.
+  - move => [S aNSR]. 
+    apply/(Requi (swap (fresh (support x)) (fresh ((support x) :|: S)))).
+    rewrite swapL [_ \dot x]fresh_transp ?fresh_notin ?fresh_subsetnotin ?fsubsetUl //.
+    apply/aNSR/fresh_subsetnotin. by rewrite fsubsetUr.
+  - move => Rfresh. exists (fresh (support x)) => //. by apply fresh_notin.
+  - move => [a a_fresh_x rax] a' a'_fresh_x.
+    case: (eqVneq a a'); first by move <-.
+    move => aa'. 
+    rewrite -[a'](tfinpermL a a') -[x](fresh_transp a_fresh_x a'_fresh_x) //. 
+    by apply Requi.
 Qed.
 
 Lemma new_forall (R : atom -> X -> Prop) :
-  equivariant_set R ->
+  equivariant_prop R ->
   forall x : X, ((\new a, R a x) <-> (forall a, a # x -> R a x)).
 Proof.
 move=> Requi x. have [? ne ef] := some_any Requi x. 
@@ -688,10 +865,19 @@ by split => // /ne /ef.
 Qed.
 
 Lemma new_exists  (R : atom -> X -> Prop) :
-  equivariant_set R -> 
+  equivariant_prop R -> 
   forall x : X, ((\new a, R a x) <-> (exists2 a, a # x & R a x)).
 Proof.
-by move=> Requi x; have [fn nh ef] := some_any Requi x; split=> [/nh|/ef].
+move=> Requi x; have [fn nf nh ef] := some_any Requi x.
+by split => [/nf/nh|/ef].
+Qed.
+
+Lemma fresh_new (R : atom -> X -> Prop) :
+  equivariant_prop R ->
+  forall x: X, R (fresh (support x)) x <-> \new a, R a x. 
+Proof.
+move=> Requi x. have [fn nf nh ef] := some_any Requi x. 
+by split => [/nh/ef/fn | /nf]. 
 Qed.
 
 End SomeAny.
@@ -701,21 +887,19 @@ Notation "\new a , P" := (new (fun a:atom => P))
 Notation "a # x" := (a \notin support x)
                       (at level 0).
 
-Section NominalLambdaTerms.
+Section NominalRawLambdaTerms.
 
 Inductive rawterm : Type :=
 | rVar of atom
 | rApp of rawterm & rawterm
 | rLambda of atom & rawterm.
 
-Fixpoint termact (π : finPerm) t :=
+Fixpoint rawtermact (π : finPerm) t :=
   match t with
     |rVar a => rVar (π a)
-    |rApp t1 t2 => rApp (termact π t1) (termact π t2)
-    |rLambda a t => rLambda (π a) (termact π t)
+    |rApp t1 t2 => rApp (rawtermact π t1) (rawtermact π t2)
+    |rLambda a t => rLambda (π a) (rawtermact π t)
   end.
-
-Local Notation "π \dot t" := (termact π t). (* à supprimer *)
 
 Fixpoint term_support t :=
   match t with
@@ -757,27 +941,28 @@ Canonical rawterm_choiceType := ChoiceType rawterm rawterm_choiceMixin.
 Definition rawterm_countMixin := CanCountMixin rawterm_codeK.
 Canonical rawterm_countType := CountType rawterm rawterm_countMixin.
 
-Lemma termact1 : termact 1 =1 id.
+Lemma rawtermact1 : rawtermact 1 =1 id.
 Proof.
 elim => [a | t1 iht1 t2 iht2| a t iht]; 
 by rewrite /= ?finsfun1 ?iht1 ?iht2 ?iht.
 Qed.
 
-Lemma termactM π π' t : termact (π * π') t = termact π (termact π' t).
+Lemma rawtermactM π π' t : rawtermact (π * π') t = rawtermact π (rawtermact π' t).
 Proof.
 elim: t => [a | t1 iht1 t2 iht2 | a t iht]; 
 by rewrite /= ?finsfunM ?iht1 ?iht2 ?iht.
 Qed.
 
-Lemma termactproper : forall t1 t2 π, t1 = t2 -> (termact π t1) = (termact π t2).
+Lemma rawtermactproper : forall t1 t2 π, t1 = t2 -> (rawtermact π t1) = (rawtermact π t2).
 Proof. by move => t1 t2 π ->. Qed.
 
-Definition term_nominal_setoid_mixin := 
-  @PermSetoidMixin rawterm (@eq rawterm) termact termact1 termactM termactproper.   
+Definition rawterm_nominal_setoid_mixin := 
+  @PermSetoidMixin rawterm (@eq rawterm) rawtermact rawtermact1 
+                   rawtermactM rawtermactproper.   
 
 
-Lemma termact_id (π : finPerm) t :
-     (forall a : atom, a \in term_support t -> π a = a) -> termact π t = t.
+Lemma rawtermact_id (π : finPerm) t :
+     (forall a : atom, a \in term_support t -> π a = a) -> rawtermact π t = t.
 Proof.
 elim: t => [a |t1 iht1 t2 iht2|a t iht] /= Hsupp.
   - rewrite  Hsupp //. by rewrite in_fset1.
@@ -786,12 +971,12 @@ elim: t => [a |t1 iht1 t2 iht2|a t iht] /= Hsupp.
   - rewrite iht ?Hsupp // ?fset1U1 // => b bsuppt. by apply/Hsupp/fset1Ur.
 Qed.
 
-End NominalLambdaTerms.
+End NominalRawLambdaTerms.
 
-Definition term_nominal_mixin :=
-  @NominalMixin rawterm_choiceType term_nominal_setoid_mixin _ termact_id.
+Definition rawterm_nominal_mixin :=
+  @NominalMixin rawterm_choiceType rawterm_nominal_setoid_mixin _ rawtermact_id.
 
-Canonical term_nominalType := @NominalType rawterm_choiceType term_nominal_mixin.
+Canonical rawterm_nominalType := @NominalType rawterm_choiceType rawterm_nominal_mixin.
 
 Section AlphaEquivalence.
 
@@ -802,19 +987,22 @@ Fixpoint raw_depth (t : rawterm) : nat :=
     | rLambda _ t => (raw_depth t).+1
   end.
 
+Lemma raw_depth0var t : raw_depth t = 0 -> exists x, t = rVar x.
+Proof. case: t => // a _. by exists a. Qed.
+
 Lemma raw_depth_perm (π : finPerm) t : raw_depth (π \dot t) = raw_depth t.
 Proof. by elim: t => [x|u ihu v ihv|x u ihu] //=; rewrite ?ihu ?ihv. Qed.
 
-Lemma strong_termsupport (t : term_nominalType) : 
-  forall π, π \dot t = t -> (forall a : atom, a \in support t -> π a = a).
+Lemma strong_termsupport (t : rawterm_nominalType) : 
+  forall π, π \dot t = t -> (forall a : atom, a \in support t -> π a == a).
 Proof.
 elim: t => [a π πa_eq_a b|t iht u ihu π eq_tu a|a t iht π eq_at b].
-  - rewrite in_fset1 => /eqP ->. by case: πa_eq_a.
+  - rewrite in_fset1 => /eqP ->. by case: πa_eq_a => ->.
   - rewrite in_fsetU => /orP; case.
       apply iht; by case: eq_tu.
     apply ihu; by case: eq_tu.
   - rewrite in_fset1U => /orP; case.
-      by move/eqP ->; case: eq_at.
+      by move/eqP ->; case: eq_at => /eqP.
     apply iht; by case: eq_at.
 Qed.
 
@@ -827,25 +1015,36 @@ Fixpoint alpha_rec n t1 t2 :=
       | n, rVar a1, rVar a2 => a1 == a2
       | S n, rApp u v, rApp u' v' => alpha_rec n u u' && alpha_rec n v v'
       | S n, rLambda a u, rLambda a' u' => 
-       let a'' := fresh (support a :|: support a' :|: support u :|: support u') in 
-       alpha_rec n (swap a a'' \dot u) 
-             (swap a' a'' \dot u')
+       let z := fresh (support a :|: support u :|: (support a' :|: support u')) in 
+       alpha_rec n (swap a z \dot u) 
+             (swap a' z \dot u')
       |_, _, _ => false
   end.
 
 Definition alpha t t' := alpha_rec (raw_depth t) t t'.
 
-(*
 Lemma alpha_recE n t t' : (raw_depth t <= n) -> alpha_rec n t t' = alpha t t'.
 Proof.
 rewrite /alpha; move: {-2}n (leqnn n).
 elim: n t t' => //= [|n ihn] [x|u v|x u] [y|u' v'|y u'] [|m] //=.
   rewrite !ltnS geq_max => lmn /andP [um vm]. 
-  rewrite !ihn //. ?(leq_maxl, leq_maxr) ?geq_max
+  rewrite !ihn // ?(leq_maxl, leq_maxr) ?geq_max
              ?(leq_trans um, leq_trans vm) //.
-by rewrite !ltnS => lmn um; rewrite ihn // ?pre_depth_perm //.
+rewrite !ltnS => lmn um. by rewrite ihn // ?raw_depth_perm. 
 Qed.
-*)
+
+Lemma alpha_VarE x y : alpha (rVar x) (rVar y) = (x == y).
+Proof. by rewrite/alpha /=. Qed.
+
+Lemma alpha_appE t u t' u' : 
+  alpha (rApp t u) (rApp t' u') = alpha t t' && alpha u u'.
+Proof. by rewrite/alpha /= !alpha_recE // ?leq_maxl ?leq_maxr. Qed.
+
+Lemma alpha_lamE x t y u : 
+  alpha (rLambda x t) (rLambda y u) = 
+  let z := fresh (support x :|: support t :|: (support y :|: support u)) in
+  alpha (swap x z \dot t) (swap y z \dot u).
+Proof. by rewrite /alpha /= raw_depth_perm. Qed.
 
 Inductive alpha_spec t1 t2 : rawterm -> rawterm -> bool -> Type :=
   | AlphaVar a & t1 = rVar a & t2 = rVar a: alpha_spec t1 t2 (rVar a) (rVar a) true
@@ -908,48 +1107,781 @@ Qed.
 
 *)
 
-Lemma equi_alpha (t t' : term_nominalType) π : alpha t t' = alpha (π \dot t) (π \dot t').
+Lemma alpha_equivariant (t t' : rawterm_nominalType) π :
+  alpha (π \dot t) (π \dot t') = alpha t t'.
 Proof.
 rewrite /alpha raw_depth_perm.
 move: {-1}(raw_depth t) (leqnn (raw_depth t)) => n.
 elim: n t t' π => [|n ihn] [x|u v|x u] [y|u' v'|y u'] π //=;
-  do ?by rewrite -(inj_eq (@finperm_inj π)). 
+  do ?by rewrite (inj_eq (@finperm_inj π)). 
   rewrite ltnS geq_max => /andP [un vn] //. rewrite (ihn _ _ π)//.
-  by rewrite [_ v v'](ihn _ _ π).
+  by rewrite -[_ v v'](ihn _ _ π).
 rewrite ltnS.
-set a := fresh _. set a' := fresh _.
+set a' := fresh _. set a := fresh _.
 rewrite -[a'](finpermVK π) -!actM -!tfinperm_conj => ru_lt_n. 
 have u_fix : swap a (π^-1 a') \dot u = u.
-  apply/fresh_transp. apply/fresh_subsetnotin/fsubset_prf. 
-  rewrite mem_im_supp;
-    last by move => π' x'; apply strong_termsupport.
-  by rewrite finperm_invK; apply/fresh_subsetnotin/fsubset_prf.
+  apply/fresh_transp. apply/fresh_subsetnotin/fsubsetU. 
+  rewrite fsubsetU // fsubsetAA orbT //. rewrite mem_im_supp;
+    last by move => x' π'; apply strong_termsupport.    
+  apply fresh_subsetnotin.
+  rewrite finperm_invK fsubsetU // fsubsetU // fsubsetAA orbT //. 
 have u'_fix : swap a (π^-1 a') \dot u' = u'.
-  apply/fresh_transp. apply/fresh_subsetnotin/fsubset_prf. 
-  rewrite mem_im_supp; 
+  apply/fresh_transp. apply/fresh_subsetnotin/fsubsetU. 
+  rewrite fsubsetUr // orbT //. rewrite mem_im_supp; 
     last by move => π' x'; apply strong_termsupport.    
-   by rewrite finperm_invK; apply/fresh_subsetnotin/fsubset_prf.
-symmetry; rewrite -{2}u_fix -{2}u'_fix (ihn _ _ (π^-1)) ?raw_depth_perm //.
+  apply fresh_subsetnotin. rewrite finperm_invK fsubsetU // fsubsetUr // orbT //.
+rewrite -{2}u_fix -{2}u'_fix -(ihn _ _ (π^-1)) ?raw_depth_perm //.
 rewrite -!actM finperm_mulA finperm_mulA !finperm_invP !finperm_oneP. 
-rewrite (ihn _ _ (swap a (π^-1 a'))) ?raw_depth_perm //.
+rewrite -(ihn _ _ (swap a (π^-1 a'))) ?raw_depth_perm //.
 rewrite -!actM tfinperm_conj [_ * swap y _]tfinperm_conj !tfinpermR !tfinpermNone //
 -finperm_can2eq !fresh_neq // in_fsetU in_fsetU in_fsetU ?in_fset1 eqxx ?orbT //.
 Qed.
 
+Lemma alpha_equivariantprop : equivariant_prop alpha.
+Proof. move => π t t' /=. by rewrite alpha_equivariant. Qed.
+
+Lemma alpha_lamP x t y u : 
+  reflect (\new a, alpha (swap x a \dot t) (swap y a \dot u))
+          (alpha (rLambda x t) (rLambda y u)).
+Proof.
+move : (equi_funprop (@swap_equiv rawterm_nominalType) alpha_equivariantprop) =>
+ /= Requi.
+apply (iffP idP).
+  rewrite alpha_lamE /= => xtαyu. 
+  by apply (fresh_new Requi ((x,t),(y,u))). 
+move/(fresh_new Requi ((x,t), (y, u))); by rewrite alpha_lamE.
+Qed.
+
+Lemma alpha_refl : reflexive alpha.
+Proof.
+rewrite /alpha.
+elim =>[a|t iht u ihu|a t iht] //=.
+  rewrite !alpha_recE ?leq_maxl ?leq_maxr /alpha //. by apply/andP.
+by rewrite alpha_recE ?raw_depth_perm ?alpha_equivariant.
+Qed.
+
+Lemma alpha_sym : symmetric alpha.
+Proof.
+move => t u; rewrite/alpha.
+move: {-1}(raw_depth t) (leqnn (raw_depth t)) => n.
+elim: n t u => [|n ihn] [x|t1 u1|x t] [y|t2 u2|y u] //=.
+  rewrite ltnS geq_max => /andP [t1_lt_n u1_lt_n].
+  by rewrite !ihn // !alpha_recE ?leq_maxl ?leq_maxr //.
+rewrite ltnS => t_lt_n.
+by rewrite ihn raw_depth_perm // fsetUC.
+Qed.
+
+Lemma alpha_trans : transitive alpha.
+Proof.
+move => u t v.
+move: {-1}(raw_depth t) (leqnn (raw_depth t)) => n.
+elim: n t u v => [|n ihn] [x|t1 u1|x t] [y|t2 u2|y u] [z|t3 u3|z v]//=;
+  do ?(move=> _ ;apply eq_op_trans).
+  rewrite ltnS geq_max !alpha_appE => /andP [t1_lt_n u1_lt_n] /andP [t1αt2] [u1αu2]
+    /andP [t2αt3 u2αu3].
+  apply/andP; split. 
+    apply (ihn _ t2) => //.
+  by apply (ihn _ u2).
+rewrite ltnS => t_lt_n.
+move => /alpha_lamP [S HS] /alpha_lamP [S' HS'].
+apply/alpha_lamP. exists (S :|: S') => a.
+rewrite in_fsetU => /norP [aNS aNS'].
+apply (ihn _ (swap y a \dot u)); first by rewrite raw_depth_perm.
+  exact: HS.
+exact: HS'.
+Qed.
+
+Canonical alpha_equiv := 
+  EquivRel alpha alpha_refl alpha_sym alpha_trans.
+
+Definition term := {eq_quot alpha}.
+Definition term_eqMixin := [eqMixin of term].
+Canonical term_eqType := EqType term term_eqMixin.
+Canonical term_choiceType := Eval hnf in [choiceType of term].
+Canonical term_countType := Eval hnf in [countType of term].
+Canonical term_quotType := Eval hnf in [quotType of term].
+Canonical term_eqQuotType := Eval hnf in [eqQuotType alpha of term].
+
+(* conflit avec fingroup *)
+Notation repr := generic_quotient.repr.
+
+(* Inductive term := *)
+(*   |BVar : nat ->  term *)
+(*   |FVar : atom -> term *)
+(*   |App : term -> term -> term *)
+(*   |Lambda : term -> term. *)
+
+(* Fixpoint open_rec (k : nat) (u : term) (t : term) {struct t} : term := *)
+(*   match t with *)
+(*     | BVar i => if k == i then u else (BVar i) *)
+(*     | FVar x  => FVar x *)
+(*     | Lambda t  => Lambda (open_rec (k.+1) u t) *)
+(*     | App t1 t2 => App (open_rec k u t1) (open_rec k u t2) *)
+(*   end. *)
+
+(* Definition open t u := open_rec 0 u t. *)
+
+(* Notation "{ k ~> u } t" := (open_rec k u t) (at level 67). *)
+(* Notation "t ^^ u" := (open t u) (at level 67). *)
+(* Notation "t ^ x" := (open t (FVar x)). *)
+
+(* Eval compute in open (App (Lambda (App (BVar 1) (BVar 0))) (BVar 0)) (FVar 7). *)
+
+(* Fixpoint pi (t : rawterm) : term := *)
+(*   let fix aux (l : seq atom) (u : rawterm) := *)
+(*       match u with  *)
+(*         |rVar x => if x \in l then BVar (index x l) else FVar (addn x (size l)) *)
+(*         |rApp t1 t2 => App (aux l t1) (aux l t2) *)
+(*         |rLambda x u' => Lambda (aux (x::l) u') *)
+(*       end *)
+(*         in *)
+(*   aux [::] t. *)
+
+(* Lemma rAppK t1 t2 : pi (rApp t1 t2) = App (pi t1) (pi t2). *)
+(* Proof. by elim: t1; elim: t2 => //. Qed. *)
+
+(* Fixpoint fvars (t : term) : seq atom := *)
+(*   match t with *)
+(*       |BVar x => [::] *)
+(*       |FVar x => [::x] *)
+(*       |App t1 t2 => (fvars t1) ++ (fvars t2) *)
+(*       |Lambda t => fvars t *)
+(*       end. *)
+
+(* Fixpoint depth (t : term) : nat := *)
+(*   match t with *)
+(*       |BVar n => 0 *)
+(*       |FVar x => 0 *)
+(*       |App t1 t2 => (maxn (depth t1) (depth t2)).+1 *)
+(*       |Lambda t => (depth t).+1 *)
+(*   end. *)
+
+(* Fixpoint wf_rec n (t : term) :=  *)
+(*   let z := fresh_list (fvars t) in  *)
+(*       match n, t with *)
+(*         |_, BVar m => false *)
+(*         |_, FVar x => true *)
+(*         |S n, App t1 t2 => (wf_rec n t1) && (wf_rec n t2) *)
+(*         |S n, Lambda t => wf_rec n (t^z) *)
+(*         |_,_ => false *)
+(*       end. *)
+
+(* Definition wf (t : term) := wf_rec (depth t) t. *)
+
+(* Lemma wf_recE n t : (depth t <= n) -> wf_rec n t = wf t. *)
+(* Proof. *)
+(* rewrite /wf; move: {-2}n (leqnn n). *)
+(* elim: n t => //= => [t n|n IH [m|x|t1 t2|t]].  *)
+(*   by rewrite leqn0 => /eqP ->; rewrite leqn0 => /eqP ->. *)
+(* rewrite /=.                *)
+(*   rewrite !ltnS geq_max => lmn /andP [um vm].  *)
+(*   rewrite !ihn // ?(leq_maxl, leq_maxr) ?geq_max *)
+(*              ?(leq_trans um, leq_trans vm) //. *)
+(* rewrite !ltnS => lmn um. by rewrite ihn // ?raw_depth_perm.  *)
+(* Qed. *)
+
+
+
+(* Lemma wf_app t1 t2 : wf (App t1 t2) = (wf t1 && wf t2). *)
+(* Proof. *)
+(* move: {-1}(depth (App t1 t2)) (leqnn (depth (App t1 t2))) => n. *)
+(* elim : n t1 t2 => [t1 t2|n IH t1 t2]. *)
+(*   by rewrite ltn0. *)
+
+
+
+(* Definition wf_term := sig wf. *)
+(* Coercion wf_term_term (t : wf_term) : term := (val t). *)
+
+(* Fixpoint repr (t : wf_term) : rawterm := *)
+(*   let fix aux (t : term) (l : seq atom) (bvars : seq atom) := *)
+(*       match t with  *)
+(*         |BVar x => rVar (nth x bvars x) *)
+(*         |FVar x => rVar x *)
+(*         |App t1 t2 => rApp (aux t1 l bvars) (aux t2 l bvars) *)
+(*         |Lambda t => let x := (fresh_list l) in rLambda x (aux t (x::l) (x::bvars)) *)
+(*       end *)
+(*   in aux t (fvars t) [::]. *)
+
+(* Lemma wf_pi (t : rawterm) : wf (pi t). *)
+(* Proof. *)
+(* elim: t => //. *)
+(*  move => t wft u wfu. rewrite rAppK. rewrite /=. *)
+
+(* Lemma reprK : cancel repr pi. *)
+(* Proof. *)
+(* elim => [a|||].  *)
+(* move => t. *)
+
+    
+Lemma alpha_eqE t t' : alpha t t' = (t == t' %[mod term]).
+Proof. by rewrite piE. Qed.
+
+Definition Var x := lift_cst term (rVar x).
+Canonical pi_Var x := PiConst (Var x). 
+
+Definition App := lift_op2 term rApp.
+Lemma rAppK : {morph \pi_term : t t' / rApp t t' >-> App t t'}.
+Proof.
+unlock App => x y /=; apply/eqP.
+by rewrite [_ == _]piE alpha_appE !alpha_eqE !reprK !eqxx.
+Qed.
+Canonical pi_App := PiMorph2 rAppK.
+
+Definition Lambda x := lift_op1 term (rLambda x).
+Lemma rLambdaK x : {morph \pi_term : u / rLambda x u >-> Lambda x u}.
+Proof.
+move => u; unlock Lambda => /=. apply/eqmodP => /=.
+by rewrite alpha_lamE //= alpha_equivariant alpha_eqE reprK. 
+Qed.
+Canonical pi_Lambda x := PiMorph1 (rLambdaK x).
+
+Lemma rVarK x : \pi_term (rVar x) = Var x.
+Proof. by rewrite !piE. Qed.
+
+Lemma VarK x : repr (Var x) = rVar x. 
+Proof.
+have: alpha (repr (Var x)) (rVar x) by rewrite alpha_eqE reprK piE.
+by case: (repr (Var x)) => //= m /eqP->.
+Qed.
+
+Lemma AppK u v : exists u' v',
+    [/\ u = \pi_term u', v = \pi_term v' & repr (App u v) = rApp u' v'].
+Proof.
+have: alpha (repr (App u v)) (rApp (repr u) (repr v)).
+  by rewrite alpha_eqE reprK -[u]reprK -[v]reprK !piE !reprK.
+case: (repr (App _ _)) => //= u' v'; rewrite alpha_appE //.
+by rewrite !alpha_eqE !reprK => /andP [/eqP <- /eqP <-]; exists u'; exists v'; split.
+Qed.
+
+Lemma Var_inj x y : Var x = Var y -> x = y.
+Proof.
+rewrite !piE => /eqP. 
+by rewrite -alpha_eqE alpha_VarE => /eqP. 
+Qed.
+
+Lemma App_inj t1 t2 u1 u2 : 
+  App t1 t2 = App u1 u2 -> t1 = u1 /\ t2 = u2.
+Proof.
+move/(congr1 repr). 
+have [reprt1 [reprt2 [-> ->]] ->] := AppK t1 t2.
+have [repru1 [repru2 [-> ->]] ->] := AppK u1 u2.
+move => t1t2_eq_u1u2.
+by injection t1t2_eq_u1u2 => -> ->. 
+Qed.
+
 End AlphaEquivalence.
 
-(* Lemma alphaP t t' : reflect (alpha_spec t t') (alpha t t'). *)
-(* Proof. *)
-(* apply: (equivP idP). *)
-(* case: t; case: t' => //=; rewrite /alpha /=; *)
-(*   try solve [move => *; split => // H; inversion H].                            *)
-(*   - move => x y; split => [|H]. *)
-(*       by move/eqP ->; constructor. *)
-(*     by apply/eqP; inversion H.  (* comment éviter inversion ?*) *)
-(*   - move => u' v' u v. *)
+(* conflit avec fingroup *)
+Notation repr := generic_quotient.repr.
 
-(* move => /alpha_ind E. elim/E : {t t' E} _ => [x | u v u' v' _ uαu' _ vαv' |]. *)
-(*   - by rewrite/alpha /=.  *)
-(*   - rewrite/alpha /=.  *)
-(* End NominalLambdaTerms. *)
+Section NominalTerm.
+
+Implicit Types (π : finPerm) (t : term).
+
+Definition termact π t := \pi_term (π \dot repr t).
+
+Lemma termact1 : termact 1 =1 id.
+Proof. move => t /=. by rewrite /termact act1 reprK. Qed.
+
+Lemma termact_equiv π t : 
+  π \dot (repr t) == repr (termact π t) %[mod term].   
+Proof.
+rewrite /termact. rewrite reprK. done.
+Qed.
+
+Lemma termactM π π' t : termact (π * π') t = termact π (termact π' t).
+Proof.
+apply/eqP. 
+by rewrite /termact actM piE alpha_equivariant alpha_eqE reprK. 
+Qed.
+
+Lemma termactproper : 
+  forall t1 t2 π, t1 = t2 -> (termact π t1) = (termact π t2).
+Proof. by move => t1 t2 π ->. Qed.
+
+Definition term_nominal_setoid_mixin :=
+  @PermSetoidMixin term (@eq term) termact termact1 termactM termactproper.
+
+Lemma termact_id (π : finPerm) t :
+     (forall a : atom, a \in term_support (repr t) -> π a = a) -> 
+     termact π t = t.
+Proof.
+rewrite/termact => Hact_id. 
+suff : π \dot repr t = repr t by move ->; exact: reprK.
+by apply act_id. 
+Qed.
+
+Definition term_nominal_mixin :=
+  @NominalMixin term_choiceType term_nominal_setoid_mixin _ termact_id.
+
+Canonical term_nominalType := @NominalType term_choiceType term_nominal_mixin.
+
+Lemma pi_equivariant π u : π \dot (\pi_term u) = \pi_term (π \dot u).
+Proof.
+apply/eqmodP => /=. 
+by rewrite alpha_equivariant alpha_eqE reprK. 
+Qed.
+
+Lemma repr_equivariant π t : repr (π \dot t) == π \dot (repr t) %[mod term]. 
+Proof. by rewrite -pi_equivariant !reprK. Qed.
+
+Lemma eq_lam x t y u : 
+  x # (y,u) -> (t = swap x y \dot u) ->
+  Lambda x t = Lambda y u.                                                  
+Proof.
+rewrite in_fsetU /= in_fset1 => /norP [x_neq_y x_fresh_t] ->.
+unlock Lambda; apply/eqP; rewrite -alpha_eqE alpha_lamE /= alpha_eqE. 
+set z := fresh _.
+rewrite -!pi_equivariant !reprK.
+have xzu : swap x z \dot u = u.  
+  apply/fresh_transp => //; apply/fresh_subsetnotin.
+  by rewrite fsetUC fsubsetU // fsubsetUr.
+rewrite -{2}xzu -!actM tfinperm_conj tfinpermL tfinpermNone ?[_ z y]tfinpermC//.
+rewrite fresh_neq; first by rewrite eq_sym x_neq_y.
+by rewrite fsetUC in_fsetU in_fsetU in_fset1 eqxx.
+Qed.
+
+Lemma Var_equiv π u : π \dot (Var u) = Var (π \dot u).
+Proof. by rewrite -rVarK pi_equivariant /= rVarK. Qed.
+
+Lemma App_equiv π t u : π \dot (App t u) = App (π \dot t) (π \dot u).
+Proof. 
+move: (rAppK (repr t) (repr u)). 
+by rewrite !reprK => <-; rewrite pi_equivariant rAppK. 
+Qed.
+
+Lemma Lam_equiv π x t : π \dot (Lambda x t) = Lambda (π \dot x) (π \dot t).
+Proof.
+move: (rLambdaK x (repr t)).
+rewrite !reprK => <-; by rewrite pi_equivariant rLambdaK. 
+Qed.
+
+Lemma fresh_var x y : x # (Var y) = (x != y).
+Proof. by rewrite /support/= VarK/= in_fset1. Qed.
+
+End NominalTerm.
+
+Section EliminationPrinciples.
+
+Lemma LambdaK x (u : term) : exists y (v : rawterm),
+    [/\ \new z, \pi (swap y z \dot v) = swap x z \dot u  & repr (Lambda x u) = rLambda y v].
+Proof.
+have: alpha (repr (Lambda x u)) (rLambda x (repr u)).
+  by rewrite alpha_eqE reprK -[u]reprK !piE !reprK.
+case: (repr (Lambda _ _)) => //= y v /alpha_lamP [S HS].
+exists y; exists v. split => //.
+exists S => z /HS.
+by rewrite alpha_eqE => /eqP.
+Qed.
+
+Lemma term_ind (P : term -> Prop) :
+  (forall x, P (Var x)) ->
+  (forall t1 t2, P t1 -> P t2 -> P (App t1 t2)) ->
+  (forall x t, P t -> P (Lambda x t)) ->
+              forall u, P u.
+Proof.
+move => HVar HApp HLam u; rewrite -[u]reprK.
+elim: (repr u) => [x|t Ht t' Ht'|a t Ht].
+  - by rewrite rVarK.
+  - rewrite rAppK. by apply HApp.
+  - rewrite rLambdaK. by apply HLam.
+Qed.
+
+Definition term_rect (P : term -> Type) :
+  (forall x, P (Var x)) ->
+  (forall t1 t2, P t1 -> P t2 -> P (App t1 t2)) ->
+  (forall x t, P t -> P (Lambda x t)) ->
+              forall u, P u.
+move => HVar HApp HLam u; rewrite -[u]reprK.
+elim: (repr u) => [x|t Ht t' Ht'|a t Ht].
+  - by rewrite rVarK.
+  - rewrite rAppK. by apply HApp.
+  - rewrite rLambdaK. by apply HLam.
+Defined.
+
+(* Lemma term_rect_VarE P x f1 f2 f3 : @term_rect P f1 f2 f3 (Var x) = f1 x. *)
+(* Proof. *)
+(* rewrite /term_rect/=. *)
+(* generalize (reprK (Var x)). generalize (repr (Var x)). generalize (Var x) at 2 4. *)
+(* apply eq_rect_dep_sym. *)
+
+(* move: (VarK x) => e. case_eq e. *)
+(* move: (rVarK x). move <-. *)
+(* elim: (repr (Var x)). *)
+(* rewrite/term_rect. *)
+(* destruct (repr (Var x)). *)
+(* rewrite VarK. rewrite reprK. *)
+
+Lemma term_altind_subproof (X : nominalType) (P : term -> X -> Prop) :
+  (forall x C, P (Var x) C) ->
+  (forall C t1 t2, (forall D, P t1 D) -> (forall D, P t2 D) -> 
+                   P (App t1 t2) C) ->
+  (forall x t C, x # C -> (forall D, P t D) -> P (Lambda x t) C) ->
+  forall u π C, P (π \dot u) C.
+Proof.
+move => HVar HApp HLam u.
+elim/term_ind : u => [x π C|t1 t2 IHt1 IHt2 π C|].
+  - rewrite Var_equiv. by apply HVar.
+  - rewrite App_equiv. by apply HApp.
+  - move => x t HPt π C.
+    rewrite Lam_equiv. have [xfreshC | xNfreshC] := boolP ((π \dot x) # C).
+      by apply HLam.
+    pose z := fresh (support C :|: support (π \dot x) :|: support (π \dot t)).
+    suff : (Lambda (π \dot x) (π \dot t)) = 
+           (Lambda z (swap (π \dot x) z \dot (π \dot t))).
+      move->; apply HLam; [|rewrite -actM; exact: HPt]. 
+      apply/fresh_subsetnotin. by rewrite -fsetUA fsubsetUl.
+    apply/sym_eq/eq_lam; last by rewrite tfinpermC.
+    apply fresh_subsetnotin. by rewrite -fsetUA fsubsetUr.
+Qed.
+
+Lemma term_altind (X : nominalType) (P : term -> X -> Prop) C :
+  (forall x C, P (Var x) C) ->
+  (forall C t1 t2, (forall D, P t1 D) -> (forall D, P t2 D) -> 
+                   P (App t1 t2) C) ->
+  (forall x t C, x # C -> (forall D, P t D) -> P (Lambda x t) C) ->
+  forall u, P u C.
+Proof. 
+move => HVar HApp HLam u. rewrite -[u]act1 => *. 
+exact: term_altind_subproof. 
+Qed.
+
+
+(* freshness condition for binders *)
+Definition FCB_supp (X : nominalType) (S : {fset atom}) (f : atom ->  term -> X -> X) :=
+  forall a t r, a # S -> a # (f a t r).
+
+Definition FCB (X : nominalType) (f : atom -> term -> X -> X) :=
+  exists S, FCB_supp S f.
+
+Variables (X : nominalType) (f1 : atom -> X)
+          (f2 : term -> term -> X -> X -> X) 
+          (f3 : atom -> term -> X -> X)
+          (S1 S2 S3 : {fset atom}).
+
+Hypothesis finsupp_f1 : function_support1 f1 S1.
+Hypothesis finsupp_f2 : function_support4 f2 S2.
+Hypothesis finsupp_f3 : function_support3 f3 S3.
+Hypothesis FCB_f3 : FCB_supp S3 f3. 
+
+Definition depth (t : term) := (raw_depth (repr t)).
+
+Lemma raw_depthα_subproof :
+  forall n t1 t2, raw_depth t1 <= n -> 
+            alpha t1 t2 -> raw_depth t1 = raw_depth t2.
+Proof.
+elim => [t1 t2|n IHn t1 t2]. 
+  rewrite leqn0 => /eqP /raw_depth0var [x ->].  
+  by case: t2.
+case: t1; case: t2 => //.
+  move => t1 t2 u1 u2 /=. 
+  rewrite ltnS /= alpha_appE geq_max => /andP [u1n u2n] /andP [u1t1 u2t2]. 
+  by rewrite (IHn u1 t1) // (IHn u2 t2).
+move => x t y u /=.
+rewrite ltnS alpha_lamE /=. 
+set z := fresh _.
+rewrite -(raw_depth_perm (swap y z)) /= => u_n uαt. 
+by rewrite (IHn _ (swap x z \dot t) u_n) ?raw_depth_perm.
+Qed.
+
+Lemma raw_depthα t1 t2 :
+  alpha t1 t2 -> raw_depth t1 = raw_depth t2.
+Proof.
+exact: (raw_depthα_subproof (leqnn (raw_depth t1))).
+Qed.
+
+Lemma depth0var t : depth t = 0 -> exists x, t = Var x.
+Proof.
+rewrite/depth => /raw_depth0var [x tVarx].
+exists x.
+by rewrite -[t]reprK tVarx rVarK.
+Qed.
+
+Lemma depth_var x : depth (Var x) = 0.
+Proof. by rewrite/depth VarK. Qed.
+
+Lemma depth_perm t π : depth (π \dot t) = depth t.
+Proof.
+rewrite /depth (@raw_depthα (repr (π \dot t)) (π \dot (repr t))).
+  exact: raw_depth_perm.
+rewrite alpha_eqE. exact: repr_equivariant.
+Qed.
+
+Lemma depth_app t1 t2 : 
+  depth (App t1 t2) = (maxn (depth t1) (depth t2)).+1.
+Proof.
+have [reprt1 [reprt2 [Ht1 Ht2 reprt1t2]]] := AppK t1 t2.
+rewrite/depth reprt1t2/=.
+apply eq_S. congr maxn.
+  rewrite (@raw_depthα reprt1 (repr t1)) //.
+  by rewrite alpha_eqE -Ht1 reprK. 
+rewrite (@raw_depthα reprt2 (repr t2)) //.
+by rewrite alpha_eqE -Ht2 reprK.
+Qed.
+
+Lemma depth_lam x t :
+  depth (Lambda x t) = (depth t).+1.
+Proof.
+have [y [u [[S HS]]] repr_xt] := LambdaK x t.
+rewrite /depth repr_xt/=.
+pose z := fresh S.
+rewrite -(raw_depth_perm (swap y z)).
+rewrite -[X in _ = X.+1](raw_depth_perm (swap x z)).
+apply/eq_S/raw_depthα.
+rewrite alpha_eqE -[X in _ == X]pi_equivariant reprK.
+apply/eqP. exact: (HS z (fresh_notin S)).
+Qed.
+
+Lemma depth_repr (t : rawterm) :
+  raw_depth t = depth (\pi t).
+Proof.
+rewrite/depth. apply raw_depthα.
+by rewrite alpha_eqE reprK.
+Qed.
+
+Variable (dflt : X).
+
+Fixpoint term_altrect_rec n (t : term) :=
+  match n, repr t with 
+    |_, rVar x => f1 x
+    |S n, rApp t1 t2 => f2 (\pi t1) (\pi t2) 
+                      (term_altrect_rec n (\pi t1)) 
+                      (term_altrect_rec n (\pi t2))
+    |S n, rLambda x u => let z := fresh ((S1 :|: S2 :|: S3) :|: (support x :|: support t)) in 
+                         f3 z (\pi ((swap x z) \dot u)) 
+                            (term_altrect_rec n (\pi ((swap x z) \dot u)))
+    |_,_ => dflt
+  end.
+
+Definition term_altrect (t : term) :=
+  term_altrect_rec (depth t) t.
+
+Lemma term_altrect_recE_subproof n m t :
+  depth t <= n -> n <= m -> term_altrect_rec n t = term_altrect_rec m t.
+Proof.
+elim: m n t =>[n t tn|m IHm n t].
+  by rewrite leqn0 => /eqP ->.
+case: n => [|n].
+  rewrite leqn0 => /eqP /depth0var => [[x ->]].
+  by rewrite /= VarK.
+rewrite ltnS /=.
+case_eq (repr t) => // [t1 t2 reprt|x u repru].
+  rewrite /depth reprt /= ltnS geq_max => /andP [t1n t2n] nm.
+  have deptht1 : depth (\pi t1) <= n 
+    by rewrite -depth_repr.
+  have deptht2 : depth (\pi t2) <= n 
+    by rewrite -depth_repr.
+  by rewrite !IHm //.
+set z := fresh _.
+rewrite/depth repru /= ltnS => u_leq_n nm.
+have depthu : depth (\pi_(term) u) <= n 
+  by rewrite -depth_repr.
+congr f3.
+apply IHm => //.
+by rewrite -pi_equivariant depth_perm.
+Qed.
+
+Lemma term_altrect_recE n t :
+  depth t <= n -> term_altrect_rec n t = term_altrect t.
+Proof.
+rewrite/term_altrect => t_leq_n.
+symmetry.
+by apply term_altrect_recE_subproof.
+Qed.
+
+(* Lemma raw_fun_equivariant_subproof t (π: finPerm) : *)
+(*     [disjoint S1 & finsupp π] -> *)
+(*     [disjoint S2 & finsupp π] -> *)
+(*     [disjoint S3 & finsupp π] -> *)
+(* π \dot (raw_fun_subproof t) = raw_fun_subproof (π \dot t). *)
+(* Proof. *)
+(* elim: t => [x S1π _ _|t1 IHt1 t2 IHt2 S1π S2π S3π|x t IHt S1π S2π S3π]. *)
+(*   - exact: finsupp_f1.  *)
+(*   - rewrite /= finsupp_f2 //. *)
+(*     by rewrite IHt1 // IHt2 // !pi_equivariant. *)
+(*   - rewrite /= finsupp_f3 //. *)
+(*     by rewrite IHt // pi_equivariant. *)
+(* Qed. *)
+
+Lemma fset1_disjoint (x : atom) (A B : {fset atom}) : 
+  [disjoint x |: A & B] = ((x \notin B) && [disjoint A & B]%fset).
+Proof.
+apply/idP/idP.
+  move/fdisjointP => H; apply/andP; split.
+    apply H. by rewrite fset1U1.
+  apply/fdisjointP => a /(fsubsetP (fsubsetU1 x A) a). 
+  exact: H.
+move/andP => [xNB /fdisjointP A_disj_B]; apply/fdisjointP => a.
+rewrite in_fset1U => /orP; case.
+  by move/eqP ->.
+exact: A_disj_B.
+Qed.
+
+Lemma term_altrect_VarE x : @term_altrect (Var x) = f1 x.
+Proof. by rewrite/term_altrect/depth /= VarK /= VarK. Qed.
+
+Lemma term_altrect_AppE t1 t2 :
+  @term_altrect (App t1 t2) = 
+  f2 t1 t2 
+     (term_altrect t1)
+     (term_altrect t2).
+Proof.
+have [reprt1 [reprt2 [Ht1 Ht2 reprt1t2]]] := AppK t1 t2.
+rewrite/term_altrect depth_app /= reprt1t2  -Ht1 -Ht2. 
+by rewrite !term_altrect_recE // ?leq_maxl ?leq_maxr.
+Qed.
+
+Lemma term_altrect_equivariant t (π : finPerm) :
+  [disjoint S1 & finsupp π] ->
+  [disjoint S2 & finsupp π] ->
+  [disjoint S3 & finsupp π] ->
+  π \dot (term_altrect t) = term_altrect (π \dot t).
+Proof.
+move : {-1}(depth t) (leqnn (depth t)) => n.
+elim: n t π => [t π|n IHn t π].
+  rewrite leqn0 => /eqP /depth0var => [[x ->]] S1_π S2_π S3_π.
+  rewrite Var_equiv !term_altrect_VarE.
+  exact: finsupp_f1.
+rewrite leq_eqVlt => /orP; case =>[/eqP|]; last by
+  rewrite ltnS; exact: IHn.
+rewrite /term_altrect depth_perm => depth_t S1_π S2_π S3_π.
+rewrite depth_t /=.
+have : alpha (repr (π \dot t)) (π \dot (repr t)).
+  by rewrite alpha_eqE; exact: repr_equivariant.
+case_eq (repr t); case_eq (repr (π \dot t)) => //.
+  - move => a repr_πt b repr_t. 
+    have -> : π \dot rVar b = rVar (π \dot b) by [].
+    rewrite alpha_VarE => /eqP ->.
+    exact: finsupp_f1.
+  - move => t1 t2 _ u1 u2 repr_t.
+    have -> : π \dot (rApp u1 u2) = rApp (π \dot u1) (π \dot u2) by [].
+    rewrite alpha_appE !alpha_eqE => /andP [/eqP t1_u1 /eqP t2_u2].
+    rewrite t1_u1 t2_u2 finsupp_f2 // !pi_equivariant.
+    have depth_u1 : depth (\pi u1) = n by admit.
+    have depth_u2 : depth (\pi u2) = n by admit.
+    rewrite -{1}depth_u1 -depth_u2 -!pi_equivariant.
+    congr f2.
+       rewrite depth_u2 -depth_u1 -{2}(depth_perm _ π).
+       apply IHn => //. by rewrite depth_u1 leqnn.
+    rewrite -{2}(depth_perm _ π). apply IHn => //. by rewrite depth_u2 leqnn.
+  - move => y u repr_πt z v repr_t.
+    set a := fresh _; set b := fresh _.
+    have aNS1 : a \notin S1 by
+      apply/fresh_subsetnotin/fsubsetU/orP; left; rewrite -fsetUA fsubsetUl.
+    have aNS2 : a \notin S2 by
+      apply/fresh_subsetnotin/fsubsetU/orP; left; apply/fsubsetU; rewrite fsubsetUr.
+    have aNS3 : a \notin S3 by
+      apply/fresh_subsetnotin/fsubsetU; rewrite fsubsetUr.
+    have bNS1 : b \notin S1 by
+        apply/fresh_subsetnotin/fsubsetU/orP; left; rewrite -fsetUA fsubsetUl.
+    have bNS2 : b \notin S2 by
+        apply/fresh_subsetnotin/fsubsetU/orP; left; apply/fsubsetU; rewrite fsubsetUr.      
+    have bNS3 : b \notin S3 by
+      apply/fresh_subsetnotin/fsubsetU; rewrite fsubsetUr.
+    have -> : π \dot (rLambda z v) = rLambda (π \dot z) (π \dot v) by [].
+    move => /alpha_lamP [S HS].
+    set t1 := \pi_term _; set t2 := \pi_term _.
+    pose m := fresh ((S :|: S1) :|: (S2 :|: S3 ) :|: (support (π \dot v) :|: support u) :|:
+                     (support (f3 a t1 (term_altrect t1)) :|:
+                     (π^-1 \dot (support (f3 b t2 (term_altrect t2)))))).
+    have mNS1 : m \notin S1 by admit.
+    have mNS2 : m \notin S2 by admit.
+    have mNS3 : m \notin S3 by admit.
+    have depth_zav : n = depth (\pi (swap z a \dot v)).
+      move: (congr1 \pi_term repr_t) => /(congr1 depth).
+      rewrite reprK depth_t rLambdaK depth_lam -pi_equivariant depth_perm. 
+      exact: eq_add_S.
+    have depth_ybu : n = depth (\pi (swap y b \dot u)).
+      move: (congr1 \pi_term repr_πt) => /(congr1 depth).
+      rewrite reprK depth_perm depth_t rLambdaK depth_lam -pi_equivariant depth_perm. 
+      exact: eq_add_S.
+    rewrite {1}depth_zav depth_ybu.
+    rewrite -[f3 a _ _](@fresh_transp _ a m); last first.
+      apply/fresh_subsetnotin/fsubsetU/orP; right; apply fsubsetUl.     
+      by apply/FCB_f3/fresh_subsetnotin/fsubsetU; rewrite fsubsetUr.
+    rewrite finsupp_f3; last exact: tfinperm_disj.
+    rewrite swapL finsupp_f3 //. rewrite IHn; 
+      try (by apply tfinperm_disj); last first.
+      by rewrite depth_zav leqnn.
+    rewrite IHn //; last by rewrite depth_perm depth_zav leqnn.                rewrite -[RHS](@fresh_transp _ b (π m)); last first.
+      admit.
+      exact: FCB_f3.
+    rewrite finsupp_f3; last by admit.
+    rewrite swapL IHn; last first.
+      admit. admit. admit. admit.
+    suff : π \dot swap a m \dot t1 = swap b (π m) \dot t2 by move ->. 
+    have πmNS : π m \notin S by admit.
+    rewrite/t1/t2 -!pi_equivariant.
+    rewrite -[swap _ _ \dot _]actM tfinperm_conj tfinpermL tfinpermNone;
+      last by admit.
+    rewrite actM [swap a m \dot _]fresh_transp; last first.
+      admit. admit. 
+    move : (HS _ πmNS). rewrite alpha_eqE -!pi_equivariant => /eqP. 
+    rewrite -!actM tfinperm_conj => <-. 
+    rewrite tfinperm_conj tfinpermL tfinpermNone; last by admit.
+    by  rewrite actM [swap b _ \dot _]fresh_transp; last first;
+      admit; admit.
+Qed.
+
+Lemma f3α x t y u :
+  x \notin S1 :|: S2 :|: S3 -> y \notin S1 :|: S2 :|: S3 -> Lambda x t = Lambda y u ->
+  f3 x t (term_altrect t) = f3 y u (term_altrect u).
+Proof.
+move => xNS1S2S2 yNS1S2S3. 
+unlock Lambda => /eqP. rewrite -alpha_eqE => /alpha_lamP [S HS].
+pose z := fresh (S1 :|: S2 :|: S3 :|: S :|:
+                 support (f3 x t (term_altrect t)) :|:
+                 support (f3 y u (term_altrect u))).
+have zNS3 : z \notin S3 by admit.
+have xNS3 : x \notin S3 by admit.
+have yNS3 : y \notin S3 by admit.
+have <- : (f3 z ((swap x z) \dot t) ((swap x z) \dot (term_altrect t))) = (f3 x t (term_altrect t)).
+  rewrite -{1}(swapL x z) -finsupp_f3.
+    rewrite fresh_transp //; first exact: FCB_f3.
+    apply/fresh_subsetnotin/fsubsetU.
+    by rewrite fsubsetUr.
+  apply/fdisjointP => b.
+  apply contraL => /(fsubsetP (tfinperm_supp x z) b).
+  rewrite in_fset2 => /orP. case;
+    by move/eqP ->.
+have <- : (f3 z ((swap y z) \dot u) ((swap y z) \dot (term_altrect u))) = (f3 y u (term_altrect u)).
+  rewrite -{1}(swapL y z) -finsupp_f3.
+    rewrite fresh_transp //; first exact: FCB_f3.
+    apply/fresh_subsetnotin/fsubsetU.
+    by rewrite fsubsetAA orbT.
+  apply/fdisjointP => b.
+  apply contraL => /(fsubsetP (tfinperm_supp y z) b).
+  rewrite in_fset2 => /orP. case;
+    by move/eqP ->.
+rewrite !term_altrect_equivariant;
+  try (apply/fdisjointP; admit).
+suff : swap x z \dot t = swap y z \dot u by move ->.
+have zNS : z \notin S by admit. 
+move : (HS _ zNS). 
+by rewrite alpha_eqE -!pi_equivariant !reprK => /eqP.
+Qed.
+
+Lemma term_altrect_LamE x t :
+  x \notin (S1 :|: S2 :|: S3) -> 
+  @term_altrect (Lambda x t) = f3 x t (term_altrect t).
+Proof.
+rewrite in_fsetU in_fsetU => /norP [/norP [xNS1 xNS2]] xNS3.
+have [y [u [[S HS] repr_xt]]] := LambdaK x t.   
+rewrite/term_altrect depth_lam /= repr_xt.
+set a := fresh _. 
+move: (HS _ (fresh_notin S)) => yzu_xzt.
+have depth_tu : depth t = depth (\pi (swap y a \dot u)).
+  rewrite -pi_equivariant depth_perm.
+  rewrite -(depth_perm _ (swap x (fresh S))) -yzu_xzt.
+  by rewrite -pi_equivariant depth_perm.
+have aNS3 : a \notin S3 by admit.
+rewrite {1}depth_tu.
+apply f3α => //. admit. admit.
+rewrite (@eq_lam a _ y (\pi u)).
+  move: (congr1 \pi_term repr_xt).
+  by rewrite reprK rLambdaK.
+admit.
+rewrite -pi_equivariant. admit.
+Qed.
 
